refactor llcei to take whole network

raft/LeaderLogsCandidateEntriesInterface.v
@@ -14,17 +14,17 @@ Section CandidateEntriesInterface.
   Context {one_node_params : OneNodeParams orig_base_params}.
   Context {raft_params : RaftParams orig_base_params}.
 
-  Definition leaderLogs_candidateEntries sigma :=
+  Definition leaderLogs_candidateEntries net :=
     (forall h e t ll,
-       In (t, ll) (leaderLogs (fst (sigma h))) ->
+       In (t, ll) (leaderLogs (fst (nwState net h))) ->
        In e ll ->
-       candidateEntries e sigma).
+       candidateEntries e (nwState net)).
 
   Class leaderLogs_candidate_entries_interface : Prop :=
     {
       leaderLogs_candidate_entries_invariant :
         forall (net : network),
           refined_raft_intermediate_reachable net ->
-          leaderLogs_candidateEntries (nwState net)
+          leaderLogs_candidateEntries net
     }.
 End CandidateEntriesInterface.
